

$$
R_t = \frac{r_t}{\sum_{i=1}^n{\frac{y_i(e^{-r_ta_{i-1}}-e^{-r_ta_{i}})}{a_i-a_{i-1}}}} \\
R_t = \frac{r_t}{\sum_{i=1}^n{y_i(e^{-r_t(i-1)}-e^{-r_ti})}} \\
R_t = \frac{r_t}{
  \sum_{i=1}^n{y_ie^{-r_t(i-1)}-\sum_{i=1}^n{y_ie^{-r_ti}}}
} \\
R_t = \frac{r_t}{
  \sum_{j=0}^{n-1}{y_{j+1}e^{-r_tj}-\sum_{i=1}^n{y_ie^{-r_ti}}}
} \\
R_t = \frac{r_t}{
  y_1 + \sum_{j=1}^{n-1}{y_{j+1}e^{-r_tj}-\sum_{i=1}^{n-1}{y_ie^{-r_ti}}} + y_ne^{-r_tn}
} \\

R_t = \frac{r_t}{
  y_1 + \sum_{i=1}^{n-1}{(y_{i+1}-y_i)e^{-r_ti}} + y_ne^{-r_tn}
} \\
y_{n+1} = 0 \\
\Delta{y_i} = y_{i+1} - y_i \\
R_t = \frac{r_t}{
  y_1+\sum_{i=1}^{n}{\Delta{y_i}e^{-r_ti}}
} \\
$$

$M$ is moment generating function of the infectivity profile

$$
R = \frac{1}{M(-r)}\\

M(x) = 1 + x \sum_i{iy_i}+\frac{x^2}{2!}\sum_i{i^2y_i}+\frac{x^3}{3!}\sum_i{i^3y_i}+\dots \\

\sum_{i=1}^n{y_i} = 1 \\
M(x) = \sum_{j=0}^nx^j\sum_{i=1}^n\frac{i^jy_i}{j!} \\

b_j = \sum_{i=1}^n\frac{i^jy_i}{j!} \\
b_0 = 1 \\
d_0 = 1 \\
d_{n} = -\sum_{k=0}^{n-1} d_kb_{n-k} \\

M'(x) = \sum_{j=0}^nx^jd^j \\
R = M'(-r)
$$

This is a power series. Combining multiple should be possible using relationships
here: https://en.wikipedia.org/wiki/Power_series

https://math.stackexchange.com/questions/2051583/mixture-distribution-moment-generating-function


Transformation of reciprocal part can be done with this:
https://mathoverflow.net/questions/53384/power-series-of-the-reciprocal-does-a-recursive-formula-exist-for-the-coeffic
be can assume in this case that b_0=1

To get a single MGF for the combination of infectivity profiles, which could
be precalculated.

```{r}
# Infectivity profiles are 
ip = .epiestim_si(5,1,3,1, seed=100)
ip1 = ip %>% filter(cur_group_id()==1) %>% pull(probability)

# F = splinefun(0:(length(ip1)), c(0,cumsum(ip1)),method="monoH.FC")
# F(0:14)
# moment = function(m) integrate(lower = 0,upper = length(ip1), f = function(x) x^m * F(x,deriv=1))

moment(0)
moment(1)
moment(2)
moment(3)

moment = function(m) sum((1:length(ip1))^m*ip1)
b = sapply(1:length(ip1), function(i) moment(i)/factorial(i))

R_t = function(r_t) {
  1/(1+sum(sapply(1:length(b), function(j) (-r_t)^j*b[j])))
}

R_t(0.1)
R_t(0)
R_t(-0.1)


d = rep(0,length(b))
for (n in seq_along(d)) {
  d[n] = -sum(rev(b[1:n]) * c(1,d[1:(n-1)]))
}

R_t2 = function(r_t) {
  1+sum(sapply(1:length(d), function(j) (-r_t)^j*d[j]))
}

R_t2(0.1)
R_t2(-0.1)

```





